Veritas.BinTreePtr.fsti
@@ -8,10 +8,30 @@ open Veritas.BinTree
  *)
 type ptrfn = (n:bin_tree_node) -> (c:bin_tree_dir) -> option (d:bin_tree_node{is_desc d (child c n)})
 
+(* Is d descendant of a following pf pointers *)
+val is_pdesc (pf: ptrfn) (d a: bin_tree_node): Tot bool
+
+(* are a1 a2 in anc-desc relationship wrt p *)
+let is_panc_pdesc_sym (pf: ptrfn) (a1 a2: bin_tree_node): bool = 
+  is_pdesc pf a1 a2 || is_pdesc pf a2 a1
+
+(* unrelated in terms of p-anc-desc *)
+let non_panc_pdesc (pf: ptrfn) (a1 a2: bin_tree_node): bool = 
+  not (is_panc_pdesc_sym pf a1 a2)
+
+(* every node is a pdesc of itself *)
+val lemma_pdesc_reflexive (pf: ptrfn) (a: bin_tree_node):
+  Lemma (is_pdesc pf a a)
+
+(* pdesc is a transitive relation *)
+val lemma_pdesc_transitive (pf: ptrfn) (a b c: bin_tree_node):
+  Lemma (requires (is_pdesc pf a b /\ is_pdesc pf b c))
+        (ensures (is_pdesc pf a c))
+
 (* pointer based descendant relation *)
 noeq type pdesc: ptrfn -> bin_tree_node -> bin_tree_node -> Type = 
-  | PSelf: #pf: ptrfn -> n:bin_tree_node -> pdesc pf n n
-  | PTran: #pf: ptrfn -> d:bin_tree_node -> a:bin_tree_node -> _:(pdesc pf d a) -> 
+  | PSelf: pf: ptrfn -> n:bin_tree_node -> pdesc pf n n
+  | PTran: pf: ptrfn -> d:bin_tree_node -> a:bin_tree_node -> _:(pdesc pf d a) -> 
            c:bin_tree_dir{Some? (pf d c)} ->
            pdesc pf (Some?.v (pf d c)) a
 
