Veritas.SparseMerkle.fst
@@ -1,0 +1,3 @@
+module Veritas.SparseMerkle
+
+let hashfn (m:merkle_payload): hash_value = admit()
